\chapter{Fourier Series and Integrals}
\section{Fourier coefficients and series}

\question
\begin{enumerate}
\item {}(Page 1)
How to use Euler's indentity
\begin{equation*}
    e^{ikx}
    =
    \cos(kx)+
    \imath \sin(kx)
\end{equation*}
transform 
\begin{equation}
    f(x)
    =
    \sum_{k=o}^{\infty}
    a_k\cos (kx)
    +
    b_k \sin(kx)
\end{equation}
to 
\begin{equation}
    f(x)=
    \sum_{k=-\infty}^{\infty}
    c_k e^{2\pi \imath kx}
\end{equation}
?

\item {}(Page3)
Prove
\begin{equation*}
    D_N(t)
    =
    \sum_{k=-N}^{N}
    e^{2\pi\imath kt}
    =
    \frac{
        \sin(\pi(2N+1)t)
    }
    {
        \sin(\pi t)
    }.
\end{equation*}

\end{enumerate}


\solution
\begin{enumerate}
\item {}
Roughly note that 
\begin{equation*}
\begin{cases}
    c_k+c_{-k}&=a_k\\
    \imath c_k-\imath c_{-k}&=b_k
\end{cases}
\end{equation*}
Of couse , I should transform $f(x)$ to $f(\frac{x}{2\pi})$ to make period of $f$ 1.

\item {}
\begin{proof}
\begin{equation*}
\begin{aligned}
    D_N (t)=\sum_{k=-N}^{N}
    e^{2\pi\imath kt}
    =
    1+
    2\sum_{k=1}^{N}
    \cos(2\pi\imath kt)
\end{aligned}        
\end{equation*}
then use Euler's equation get:
\begin{align*}
    \cos(\theta)+\cos(2\theta)
    +\cdots
    +\cos(n\theta)
    &=
    \text{Re}(e^{\imath \theta}+e^{2\imath\theta}+\cdots +e^{n\imath\theta})\\
    &=
    \text{Re}
    \frac{
        e^{\imath\theta}
        (1-e^{n\imath \theta})
    }
    {1-e^{\imath\theta}}\tag{-}
\label{-}
\end{align*}
and 
\begin{align*}
    \frac{e^{\imath\theta}(1-e^{n\imath\theta})}
    {1-e^{\imath\theta}}
    &=
    \frac{
        e^{(\frac{n}{2}+1)\imath \theta}
        (
        e^{(-\frac{n}{2})\imath \theta}
        -
        e^{(\frac{n}{2})\imath \theta}
        )
    }
    {e^{\frac{1}{2}\imath\theta}(e^{-\frac{1}{2}\imath\theta}-e^{\frac{1}{2}\imath\theta})}
    \\
    &=
    e^{(\frac{n}{2}+\frac{1}{2})\imath\theta}
    \frac{-2\imath\sin(\frac{n}{2}\theta)}
    {-2\imath\sin(\frac{1}{2}\theta)}\tag{*}\label{*}
\end{align*}
then 
$$
\text{Re}\ref{*}
=\frac{\cos((\frac{n}{2}+\frac{1}{2})\imath \theta)\sin(\frac{n}{2}\theta)}{\sin(\frac{1}{2}\theta)}
$$
and take $n=N$ , $\theta=2\pi\imath t$ to \ref{-} , the conclusion is obvious.
\end{proof}
\end{enumerate}